

(1) Just prove that $h_\varepsilon^k(t)$ is continuous in $t=0$, $t=-\varepsilon$

when $t=0$,

$$\lim_{t \rightarrow 0^-} h_\varepsilon^k(t) = \varepsilon^{k(1-b)} b^{-k} \varepsilon^{kb} = \varepsilon^k b^{-k}, \quad \lim_{t \rightarrow 0^+} h_\varepsilon^k(t) = \lim_{t \rightarrow 0^+} (\varepsilon b^{-1})^k = \varepsilon^k b^{-k}$$

$$\text{Then: } \lim_{t \rightarrow 0^-} h_\varepsilon^k(t) = \lim_{t \rightarrow 0^+} h_\varepsilon^k(t);$$

when $t=-\varepsilon$,

$$\lim_{t \rightarrow -\varepsilon^-} h_\varepsilon^k(t) = 0, \quad \lim_{t \rightarrow -\varepsilon^+} h_\varepsilon^k(t) = 0$$

$$\text{Then: } \lim_{t \rightarrow -\varepsilon^-} h_\varepsilon^k(t) = \lim_{t \rightarrow -\varepsilon^+} h_\varepsilon^k(t).$$

To sum up, $h_\varepsilon^k(t)$ is continuous in $t=0$, $t=-\varepsilon$, $h_\varepsilon^k(t)$ is continuous in R .

(2) To prove $\forall t \in R, h_\varepsilon^m(t) \geq h^m(t)$, Just prove that $\Delta h(t) := h_\varepsilon^k(t) - h^k(t) \geq 0$, By definition:

$$\Delta h(t) := h_\varepsilon^k(t) - h^k(t) := \begin{cases} \Delta h_1(t) = 0, & t \leq -\varepsilon \\ \Delta h_2(t) = \varepsilon^{k(1-b)} b^{-k} (t + \varepsilon)^{kb}, & -\varepsilon < t \leq 0 \\ \Delta h_3(t) = (t + \varepsilon b^{-1})^k - t^k, & t > 0 \end{cases}$$

(i) If $t \leq -\varepsilon$, $\Delta h(t) = \Delta h_1(t) = 0 \geq 0$ is hold;

(ii) If $-\varepsilon < t \leq 0$, then $\varepsilon > 0$, $b > 0$, 且 $t + \varepsilon > 0$, 于是:

$$\Delta h(t) = \Delta h_2(t) = \varepsilon^{k(1-b)} b^{-k} (t + \varepsilon)^{kb} > 0$$

(iii) If $t > 0$, because $\varepsilon > 0$, $b > 0$, then $\varepsilon b^{-1} > 0$:

$$\Delta h(t) = \Delta h_3(t) = (t + \varepsilon b^{-1})^k - t^k > 0$$

To sum up, $\Delta h(t) := h_\varepsilon^k(t) - h^k(t) \geq 0$, then $\forall t \in R, h_\varepsilon^m(t) \geq h^m(t)$

By the construction of $h_\varepsilon^k(t)$,

(i) If $t \leq -\varepsilon$, $\lim_{\varepsilon \rightarrow 0} h_\varepsilon^k(t) = 0$ is hold;

(ii) If $-\varepsilon < t \leq 0$, then,

$$\frac{dh_\varepsilon^k(t)}{dt} = k \varepsilon^{k(1-b)} b^{1-k} (t + \varepsilon)^{kb-1},$$

Because $\varepsilon > 0$, $b > 0$, and $t + \varepsilon > 0$, then:

$$\frac{dh_\varepsilon^k(t)}{dt} = k \varepsilon^{k(1-b)} b^{1-k} (t + \varepsilon)^{kb-1} > 0$$

Namely smooth function $h_\varepsilon^k(t)$ is constant monotonous increase in $-\varepsilon < t \leq 0$, then

$$0 = h(-\varepsilon) < h_\varepsilon^k(t) \leq h(0) = \varepsilon^k b^{-k}$$

then

$$0 \leq \lim_{\varepsilon \rightarrow 0} h_\varepsilon^k(t) \leq \lim_{\varepsilon \rightarrow 0} \varepsilon^k b^{-k} = 0$$

$$\lim_{\varepsilon \rightarrow 0} h_\varepsilon^k(t) = 0 \text{ is hold.}$$

(iii) If $t > 0$:

$$\lim_{\varepsilon \rightarrow 0} h_\varepsilon^k(t) = \lim_{\varepsilon \rightarrow 0} (t + \varepsilon b^{-1})^k = t^k = h^k(t)$$

In summary, $\forall t \in R, \lim_{\varepsilon \rightarrow 0} h_\varepsilon^m(t) = h^m(t)$

(3) By the construction of $h_\varepsilon^k(t)$, notes:

$$h_\varepsilon^k(t) = \begin{cases} h_1(\varepsilon, t) = 0 & t < -\varepsilon \\ h_2(\varepsilon, t) = \varepsilon^{k(1-b)} b^{-k} (t + \varepsilon)^{kb} & -\varepsilon \leq t < 0 \\ h_3(\varepsilon, t) = (t + \varepsilon b^{-1})^k & t \geq 0 \end{cases}$$

First of all:

$$h_1(t, \varepsilon) = 0 < h_2(t, \varepsilon) \leq \varepsilon^k b^{-k} \leq h_3(t, \varepsilon)$$

Followed by:

$$\begin{aligned} \frac{dh_2(t, \varepsilon)}{d\varepsilon} &= k \varepsilon^{k(1-b)-1} b^{-k} (t + \varepsilon)^{kb-1} + k(1-b) \varepsilon^{k(1-b)-1} b^{-k} (t + \varepsilon)^{kb} \\ &= k \varepsilon^{k(1-b)-1} b^{-k} (t + \varepsilon)^{kb-1} (\varepsilon b + (1-b)(t + \varepsilon)) \\ &= k \varepsilon^{k(1-b)-1} b^{-k} (t + \varepsilon)^{kb-1} (t + \varepsilon - bt) \end{aligned}$$

Due to $\varepsilon > 0$, $b > 0$, $-\varepsilon < t \leq 0$, then:

$$\frac{dh_2(t, \varepsilon)}{d\varepsilon} > 0$$

and

$$\frac{dh_3(t, \varepsilon)}{d\varepsilon} = b^{-1} (t + \varepsilon b^{-1})^{k-1} > 0$$

In summary, smooth function $h_\varepsilon^k(t)$ is Constant monotonous increase in $\varepsilon \geq 0$ which means $0 < \varepsilon_1 < \varepsilon_2$, then $\forall t \in R, h_{\varepsilon_1}^k(t) \leq h_{\varepsilon_2}^k(t)$.

Theorem 2.2.2 if $\frac{1}{b} < k < +\infty$, $\varepsilon > 0$, $h_\varepsilon^k(t)$ is continuous differentiable, and

$$\frac{dh_\varepsilon^k(t)}{dt} = \begin{cases} 0 & t \leq -\varepsilon \\ k \varepsilon^{k(1-b)} b^{-k} (t + \varepsilon)^{kb-1} & -\varepsilon < t \leq 0 \\ k(t + \varepsilon b^{-1})^{k-1} & t > 0 \end{cases}$$

Consider the low-order penalty function

$$\hat{P}_\varepsilon^k(x, \pi) = \sum_{i=1}^m f_i(x) + \pi \sum_{i=1}^l h_\varepsilon^k(g_i(x)) + \pi \sum_{i=1}^m h_\varepsilon^k(f_i(x) - f_i(\hat{x}))$$

Theorem 2.2.3 For any $\frac{1}{b} < k < 1$, $\varepsilon > 0$, $b > 0$, and $f_i(x), i \in M$, $g_i(x), i \in I$ is

continuous, the following properties hold:

(1) $\hat{P}_\varepsilon^k(x, \pi)$ is continuous in R^n ;

(2) $\forall x \in R^n, \hat{P}_\varepsilon^k(x, \pi) \geq \hat{P}^k(x, \pi)$;

(3) $\forall x \in R^n, \lim_{\varepsilon \rightarrow 0} \hat{P}_\varepsilon^k(x, \pi) = \hat{P}^k(x, \pi)$;

(4) if $0 < \varepsilon_1 \leq \varepsilon_2$, then $\forall x \in R^n, \hat{P}_{\varepsilon_1}^k(x, \pi) \leq \hat{P}_{\varepsilon_2}^k(x, \pi), \forall x \in R^n, \hat{P}_{\varepsilon_1}^k(x, \pi) \leq \hat{P}_{\varepsilon_2}^k(x, \pi)$.

Theorem 2.2.4 If $\frac{1}{b} < k < 1$, $b > 0$, $\varepsilon > 0$, and $f_i(x), i \in M$, $g_i(x), i \in I$ is continuous differentiable, then $\hat{P}_\varepsilon^k(x, \pi)$ is continuous differentiable in R^n .

$$\nabla_x \hat{P}_\varepsilon^k(x, \pi) = \sum_{i=1}^m \nabla_x f_i(x) + \pi \sum_{i=1}^l \nabla_x h_\varepsilon^k(g_i(x)) + \pi \sum_{i=1}^m \nabla_x h_\varepsilon^k(f_i(x) - f_i(\hat{x}))$$

3 A MOSQP algorithm based on the low-order smooth penalty function

3.1 Quadratic programming sub-problem construction

For the initial value diffusion phase, we construct the following problems for each objective function of the multi-objective optimization problem:

$$\begin{aligned} (\text{P}_i) \quad & \min f_i(x), i \in M = \{1, \dots, m\} \\ \text{s.t.} \quad & g_i(x) \leq 0, i \in I = \{1, 2, \dots, a\} \end{aligned}$$

The value function we used at this stage is as: $f_i(x)$.

The search direction is obtained by solving the following quadratic planning subproblems:

$$\begin{aligned} \text{QP}_i(x^k, B^k) \quad & \min \frac{1}{2} (d^j)^T B^j d^j + \nabla f_i(x^j)^T d^j, i \in M = \{1, \dots, m\} \\ \text{s.t.} \quad & \nabla g_i(x^j)^T d + g_i(x^j) \leq 0 \quad i \in I \end{aligned}$$

For the multi-objective optimization problem Pareto optimal solution stage, we consider all the objective functions and take each iterative initial value point as the reference point \hat{x} , Constructing the problem(P2):

$$\begin{aligned} (\text{P2}) \quad & \min \sum_{i=1}^m f_i(x) \\ \text{s.t.} \quad & f_i(x) \leq f_i(\hat{x}), i \in M = \{1, \dots, m\} \\ & g_i(x) \leq 0, i \in I = \{1, 2, \dots, a\} \end{aligned}$$

The corresponding low-order penalty function is:

$$\hat{P}_\varepsilon^k(x, \pi) = \sum_{i=1}^m f_i(x) + \pi \sum_{i=1}^l h_\varepsilon^k(g_i(x)) + \pi \sum_{i=1}^m h_\varepsilon^k(f_i(x) - f_i(\hat{x}))$$

The search direction is obtained by solving the following quadratic planning subproblems: